mark-and-sweep/spec/GC.Spec.Coalesce.fst
@@ -3535,7 +3535,44 @@ val coalesce_aux_chain_dec
 let rec coalesce_aux_chain_dec g0 g start objs first_blue run_words fp all_objs =
   if Seq.length objs = 0 then admit ()
   else begin
-    let obj = Seq.head objs in
-    if is_blue obj g0 then admit ()
+    objects_nonempty_next start g0;
+    let header = read_word g0 start in
+    let wz = getWosize header in
+    let obj = f_address start in
+    f_address_spec start;
+    hd_address_spec obj;
+    let rest_start_nat = U64.v start + (U64.v wz + 1) * U64.v mword in
+    assert (obj == Seq.head objs);
+    Seq.cons_head_tail objs;
+    wosize_of_object_spec obj g0;
+    let ws = U64.v (wosize_of_object obj g0) in
+
+    let tail_sub (o: obj_addr)
+      : Lemma (Seq.mem o (Seq.tail objs) ==> Seq.mem o all_objs)
+      = mem_cons_lemma o obj (Seq.tail objs)
+    in
+    FStar.Classical.forall_intro (FStar.Classical.move_requires tail_sub);
+
+    if is_blue obj g0 then begin
+      let new_first : U64.t = if run_words = 0 then obj else first_blue in
+      let new_rw = run_words + ws + 1 in
+
+      let tail_white_inv (o: obj_addr)
+        : Lemma (Seq.mem o (Seq.tail objs) /\ is_white o g0 ==>
+                 read_word g (hd_address o) == read_word g0 (hd_address o))
+        = mem_cons_lemma o obj (Seq.tail objs)
+      in
+      FStar.Classical.forall_intro (FStar.Classical.move_requires tail_white_inv);
+
+      coalesce_heap_blue_step g0 g objs first_blue run_words fp;
+
+      if rest_start_nat < heap_size then begin
+        let next : hp_addr = U64.uint_to_t rest_start_nat in
+        Seq.lemma_tl obj (objects next g0);
+        assert (Seq.tail objs == objects next g0);
+        coalesce_aux_chain_dec g0 g next (Seq.tail objs) new_first new_rw fp all_objs
+      end
+      else admit ()
+    end
     else admit ()
   end
